code/experimental/P256/Hacl.Spec.P256.Ladder.fst
@@ -60,15 +60,24 @@ let _ml_step0 r0 r1 =
   let r1 = _point_double r1 in 
   (r0, r1)
 
-val _ml_step1: p: point_prime -> q: point_prime -> tuple2 point_prime point_prime
+val _ml_step1: p: point_nat -> q: point_nat -> tuple2 point_nat point_nat
 
 let _ml_step1 r0 r1 = 
-  let r3 = point_double r0 in 
-  let r1 = point_add r0 r1 in 
+  let r3 = _point_double r0 in 
+  let r1 = _point_add r0 r1 in 
   (r3, r1)
 
+(*changed to any size *)
+val _ml_step: k: scalar-> i: nat{i < 256} -> p: point_nat -> q: point_nat -> Tot (r: tuple2 point_nat point_nat)
 
-assume val montgomery_ladder_step0: p: point_prime -> q: point_prime -> 
+let _ml_step k i p q = 
+    let bit = ith_bit k i in 
+    let isZeroBit = eq #U64 bit (u64 0) in 
+    if isZeroBit then 
+      _ml_step0 p q 
+    else _ml_step1 p q  
+
+val montgomery_ladder_step0: p: point_prime -> q: point_prime -> 
   Tot (r: tuple2 point_prime point_prime 
     {
       let r0, r1 = r in 
@@ -94,7 +103,45 @@ assume val montgomery_ladder_step0: p: point_prime -> q: point_prime ->
       let x3D_0, y3D_0, z3D_0 = fromDomainPoint (x3_0, y3_0, z3_0) in
       let x3D_1, y3D_1, z3D_1 = fromDomainPoint (x3_1, y3_1, z3_1) in 
 
-      let r0N, r1N = _ml_step0 (pxD, pyD, pzD) (qxD, qyD, qzD) in 
+      let (x3N_0, y3N_0, z3N_0), (x3N_1, y3N_1, z3N_1) = _ml_step0 (pxD, pyD, pzD) (qxD, qyD, qzD) in 
+      x3N_0 == x3D_0 /\ y3N_0 == y3D_0 /\ z3N_0 == z3D_0 /\ x3N_1 == x3D_1 /\ y3N_1 == y3D_1 /\ z3N_1 == z3D_1 
+    }
+ )   
+    
+
+let montgomery_ladder_step0 r0 r1 = 
+  let r0 = point_add r0 r1 in 
+  let r1 = point_double r1 in 
+  (r0, r1)
+
+
+val montgomery_ladder_step1: p: point_prime -> q: point_prime -> 
+  Tot (r: tuple2 point_prime point_prime 
+    {
+      let r0, r1 = r in 
+
+      let x3_0 = felem_seq_as_nat (sub r0 0 4) in 
+      let y3_0 = felem_seq_as_nat (sub r0 4 4) in
+      let z3_0 = felem_seq_as_nat (sub r0 8 4) in 
+
+      let x3_1 = felem_seq_as_nat (sub r1 0 4) in 
+      let y3_1 = felem_seq_as_nat (sub r1 4 4) in 
+      let z3_1 = felem_seq_as_nat (sub r1 8 4) in 
+    
+      let x1 = felem_seq_as_nat (sub p 0 4) in 
+      let y1 = felem_seq_as_nat (sub p 4 4) in 
+      let z1 = felem_seq_as_nat (sub p 8 4) in 
+      
+      let x2 = felem_seq_as_nat (sub q 0 4) in 
+      let y2 = felem_seq_as_nat (sub q 4 4) in 
+      let z2 = felem_seq_as_nat (sub q 8 4) in
+    
+      let pxD, pyD, pzD = fromDomainPoint (x1, y1, z1) in 
+      let qxD, qyD, qzD = fromDomainPoint (x2, y2, z2) in 
+      let x3D_0, y3D_0, z3D_0 = fromDomainPoint (x3_0, y3_0, z3_0) in
+      let x3D_1, y3D_1, z3D_1 = fromDomainPoint (x3_1, y3_1, z3_1) in 
+
+      let r0N, r1N = _ml_step1 (pxD, pyD, pzD) (qxD, qyD, qzD) in 
       let (x3N_0, y3N_0, z3N_0) = r0N in 
       let (x3N_1, y3N_1, z3N_1) = r1N in 
     
@@ -102,4 +149,26 @@ assume val montgomery_ladder_step0: p: point_prime -> q: point_prime ->
       x3N_1 == x3D_1 /\  y3N_1 == y3D_1 /\  z3N_1 == z3D_1 
     }
  )   
-    
+
+
+(*R0 ← 0
+  R1 ← P
+  for i from m downto 0 do
+     if di = 0 then
+        R1 ← point_add(R0, R1)
+        R0 ← point_double(R0)
+     else
+        R0 ← point_add(R0, R1)
+        R1 ← point_double(R1)
+  return R0 *)
+
+
+let montgomery_ladder_step1 r0 r1 = 
+  let r1 = point_add r0 r1 in 
+  let r0 = point_double r0 in  
+  (r0, r1)
+
+(*
+
+val montgomery_ladder_step: k: scalar -> i: nat {i < 256} -> To
+*)
