code/experimental/P256/Hacl.Spec.P256.MontgomeryMultiplication.fst
@@ -48,7 +48,6 @@ let toDomain a =
 
 let lemmaFromDomain a = ()
 
-
 let lemmaToDomain a = ()
 
 
